implement transition from F_HANDSHAKE_A -> F_HANDSHAKE_B

ironfleet/src/Dafny/Distributed/Protocol/ZooKeeper/Follower.dfy
@@ -1,20 +1,22 @@
 include "Types.dfy"
-include "ZooKeeper_ZKDatabase"
+include "ZKDatabase.dfy"
 
 
 module ZooKeeper_Follower {
 import opened ZooKeeper_Types
 import opened ZooKeeper_ZKDatabase
 
-datatype FollowerState = F_HANDSHAKE | F_SYNC | F_RUNNING
 
+// config[my_id] is my own endpoint, config[leader_id] is the leader endpoint
 datatype Follower = Follower(
     my_id: nat,
     leader_id: nat,
-    config: Config, // The cluster configuration. config[my_id] is my own endpoint, config[leader_id] is the leader endpoint
+    config: Config,
     zkdb: ZKDatabase,
     state: FollowerState 
 )
+
+datatype FollowerState = F_HANDSHAKE_A | F_HANDSHAKE_B | F_SYNC | F_RUNNING
 
 predicate FollowerInit(s:Follower, my_id:nat, leader_id:nat, config:Config, zkdb: ZKDatabase)
 {
@@ -22,10 +24,30 @@ predicate FollowerInit(s:Follower, my_id:nat, leader_id:nat, config:Config, zkdb
     && s.leader_id == leader_id
     && s.config == config
     && s.zkdb == zkdb
-    && s.state == F_HANDSHAKE
+    && s.state == F_HANDSHAKE_A
 }
 
-// predicate FollowerSend(s:Follower, s':Follower, )
-
+predicate FollowerNext(s:Follower, s':Follower, ios:seq<ZKIo>) {
+    match s.state 
+        case F_HANDSHAKE_A => SendMyInfo(s, s', ios)
+        case F_HANDSHAKE_B => false // TODO
+        case F_SYNC => false  // TODO
+        case F_RUNNING => false  // TODO
 }
 
+
+/* State transition from F_HANDSHAKE_A -> F_HANDSHAKE_B */
+predicate SendMyInfo(s:Follower, s':Follower, ios:seq<ZKIo>) {
+    && s' == s.(state := F_HANDSHAKE_B)
+    && |ios| == 1
+    && 0 <= s.leader_id < |s.config|
+    && ios[0].LIoOpSend?
+    && var outbound_packet := ios[0].s;
+        && outbound_packet.dst == s.config[s.leader_id]
+        && outbound_packet.msg.FollowerInfo?
+        && outbound_packet.msg.sid == s.my_id
+        && if |s.zkdb.commitLog| == 0 
+            then outbound_packet.msg.latestZxid == NullZxid
+            else outbound_packet.msg.latestZxid == s.zkdb.commitLog[|s.zkdb.commitLog|-1]
+}
+}
